src/drf/ADRF_PF5.v
@@ -34,35 +34,1041 @@ Require Import PredStep.
 Require Import ReorderPromises2.
 
 Require Import Pred.
-Require Import DRF_PF0.
-Require Import DRF_PF1.
-Require Import DRF_PF3.
-Require Import DRF_PF4.
-Require Import Mapping.
-
-Require Import PFConsistent.
+Require Import AMemory.
+Require Import ALocal.
+Require Import AThread.
+Require Import APredStep.
+Require Import ADRF_PF0.
+Require Import ADRF_PF1.
+Require Import ADRF_PF2.
+Require Import ADRF_PF3.
+Require Import ADRF_PF4.
+Require Import AMapping.
 
 Set Implicit Arguments.
 
-Definition tgt_consistent_drf
-           lang (e0:Thread.t lang) max
-           (
+
+Definition map_ident_in_memory (f: Loc.t -> Time.t -> Time.t -> Prop)
+           (mem: Memory.t): Prop :=
+  forall loc to
+         (TS: Time.le to (Memory.max_ts loc mem)),
+    f loc to to.
+
+Definition map_ident_in_memory_bot
+           f mem
+           (MAP: map_ident_in_memory f mem)
+  :
+    mapping_map_bot f.
+Proof.
+  ii. eapply MAP. eapply Time.bot_spec.
+Qed.
+
+Lemma map_ident_in_memory_closed_timemap
+      f mem tm
+      (MAP: map_ident_in_memory f mem)
+      (CLOSED: Memory.closed_timemap tm mem)
+  :
+    timemap_map f tm tm.
+Proof.
+  ii. eapply MAP; eauto.
+  exploit CLOSED; eauto. i. des.
+  eapply Memory.max_ts_spec in x. des. eauto.
+Qed.
+
+Lemma map_ident_in_memory_closed_view
+      f mem vw
+      (MAP: map_ident_in_memory f mem)
+      (CLOSED: Memory.closed_view vw mem)
+  :
+    view_map f vw vw.
+Proof.
+  inv CLOSED. econs.
+  - eapply map_ident_in_memory_closed_timemap; eauto.
+  - eapply map_ident_in_memory_closed_timemap; eauto.
+Qed.
+
+Lemma map_ident_in_memory_closed_tview
+      f mem tvw
+      (MAP: map_ident_in_memory f mem)
+      (CLOSED: TView.closed tvw mem)
+  :
+    tview_map f tvw tvw.
+Proof.
+  inv CLOSED. econs.
+  - i. eapply map_ident_in_memory_closed_view; eauto.
+  - eapply map_ident_in_memory_closed_view; eauto.
+  - eapply map_ident_in_memory_closed_view; eauto.
+Qed.
+
+Lemma map_ident_in_memory_closed_opt_view
+      f mem vw
+      (MAP: map_ident_in_memory f mem)
+      (CLOSED: Memory.closed_opt_view vw mem)
+  :
+    opt_view_map f vw vw.
+Proof.
+  inv CLOSED; econs.
+  eapply map_ident_in_memory_closed_view; eauto.
+Qed.
+
+Lemma map_ident_in_memory_closed_message
+      f mem msg
+      (MAP: map_ident_in_memory f mem)
+      (CLOSED: Memory.closed_message msg mem)
+  :
+    msg_map f msg msg.
+Proof.
+  inv CLOSED; econs.
+  eapply map_ident_in_memory_closed_opt_view; eauto.
+Qed.
+
+Lemma map_ident_in_memory_promises
+      f mem0 mem
+      (MAP: map_ident_in_memory f mem)
+      (MAPLT: mapping_map_lt f)
+      (CLOSED: Memory.closed mem)
+      (MLE: Memory.le mem0 mem)
+  :
+    promises_map f mem0 mem0.
+Proof.
+  inv CLOSED. econs.
+  - i. esplits; eauto.
+    + eapply mapping_map_lt_non_collapsable; auto.
+    + eapply MLE in GET. eapply Memory.max_ts_spec in GET. des.
+      eapply MAP; eauto.
+    + eapply MLE in GET. eapply CLOSED0 in GET. des.
+      eapply map_ident_in_memory_closed_message; eauto.
+  - i. esplits; eauto.
+    + eapply MLE in GET. eapply Memory.max_ts_spec in GET. des.
+      eapply MAP; eauto.
+    + eapply MLE in GET. eapply MAP. etrans.
+      * eapply memory_get_ts_le; eauto.
+      * eapply Memory.max_ts_spec in GET. des. auto.
+Qed.
+
+Lemma map_ident_in_memory_memory
+      f mem
+      (MAP: map_ident_in_memory f mem)
+      (MAPLT: mapping_map_lt f)
+      (CLOSED: Memory.closed mem)
+  :
+    memory_map f mem mem.
+Proof.
+  eapply promises_map_memory_map.
+  eapply map_ident_in_memory_promises; eauto. refl.
+Qed.
+
+Lemma map_ident_in_memory_local
+      f mem lc
+      (MAP: map_ident_in_memory f mem)
+      (MAPLT: mapping_map_lt f)
+      (LOCAL: Local.wf lc mem)
+      (CLOSED: Memory.closed mem)
+  :
+    local_map f lc lc.
+Proof.
+  inv LOCAL. econs.
+  - refl.
+  - eapply map_ident_in_memory_closed_tview; eauto.
+  - eapply map_ident_in_memory_promises; eauto.
+Qed.
+
+Lemma update_map_lt (f: Time.t -> Time.t -> Prop) to fto
+      (MAPLT: mapping_map_lt_loc f)
+      (NOMAPPED: forall fts (MAPPED: f to fts), False)
+      (LEFT: forall ts fts (TS: Time.lt ts to) (MAPPED: f ts fts),
+          Time.lt fts fto)
+      (RIGHT: forall ts fts (TS: Time.lt to ts) (MAPPED: f ts fts),
+          Time.lt fto fts)
+  :
+    mapping_map_lt_loc (fun ts fts => <<ORIG: f ts fts>> \/ <<NEW: to = ts /\ fto = fts>>).
+Proof.
+  ii. des; clarify.
+  - eapply MAPLT; eauto.
+  - split; i.
+    + eapply RIGHT; eauto.
+    + destruct (Time.le_lt_dec t1 t0); auto. destruct l.
+      * eapply LEFT in H0; eauto.
+        exfalso. eapply Time.lt_strorder. etrans; eauto.
+      * inv H0. exfalso. eapply NOMAPPED; eauto.
+  - split; i.
+    + eapply LEFT; eauto.
+    + destruct (Time.le_lt_dec t1 t0); auto. destruct l.
+      * eapply RIGHT in H0; eauto.
+        exfalso. eapply Time.lt_strorder. etrans; eauto.
+      * inv H0. exfalso. eapply NOMAPPED; eauto.
+  - split; i.
+    + exfalso. eapply Time.lt_strorder; eauto.
+    + exfalso. eapply Time.lt_strorder; eauto.
+Qed.
+
+Fixpoint compressing_map (ts0 ts1: Time.t) (T: list Time.t) :=
+  match T with
+  | [] => bot2
+  | hd :: tl => (fun ts fts => ts = hd /\ fts = Time.middle ts0 ts1)
+                  \2/ compressing_map (Time.middle ts0 ts1) ts1 tl
+  end.
+
+Lemma compressing_map_spec ts0 ts1 T
+      (TS: Time.lt ts0 ts1)
+      (SORTED: times_sorted T)
+  :
+    (<<MAPLT: mapping_map_lt_loc (compressing_map ts0 ts1 T)>>) /\
+    (<<COMPLETE: forall to (IN: List.In to T), exists fto, (<<MAPPED: (compressing_map ts0 ts1 T) to fto>>)>>) /\
+    (<<BOUND: forall to fto (MAPPED: (compressing_map ts0 ts1 T) to fto),
+        (<<IN: List.In to T>>) /\ (<<TS0: Time.lt ts0 fto>>) /\ (<<TS1: Time.lt fto ts1>>)>>).
+Proof.
+  i. ginduction T.
+  - i. ss. splits.
+    + ii. clarify.
+    + i. clarify.
+    + i. clarify.
+  - i. ss. inv SORTED. exploit IHT.
+    { instantiate (1:=ts1). instantiate (1:=Time.middle ts0 ts1).
+      eapply Time.middle_spec; eauto. }
+    { eauto. }
+    i. des. clear IHT. splits.
+    + ii. des; clarify.
+      * split; i.
+        { exfalso. eapply Time.lt_strorder; eauto. }
+        { exfalso. eapply Time.lt_strorder; eauto. }
+      * eapply BOUND in MAP0. des.
+        eapply List.Forall_forall in HD; eauto. split; i.
+        { exfalso. eapply Time.lt_strorder; eauto. }
+        { exfalso. eapply Time.lt_strorder; eauto. }
+      * eapply BOUND in MAP1. des. split; i; auto.
+        eapply List.Forall_forall in HD; eauto.
+      * eapply MAPLT; eauto.
+    + i. des; clarify.
+      * esplits; eauto.
+      * eapply COMPLETE in IN. des. esplits; eauto.
+    + i. des; clarify.
+      * split; auto. eapply Time.middle_spec; auto.
+      * eapply BOUND in MAPPED. des. splits; auto.
+        etrans.
+        { eapply Time.middle_spec; eauto. }
+        { eauto. }
+Qed.
+
+Lemma shift_map_exists max ts0 ts1 (T: list Time.t)
+      (MAX: Time.le max ts0)
+      (TS: Time.lt ts0 ts1)
+  :
+    exists (f: Time.t -> Time.t -> Prop),
+      (<<COMPLETE: forall to (IN: List.In to T), exists fto, (<<MAPPED: f to fto>>)>>) /\
+      (<<SAME: forall ts (TS: Time.le ts max), f ts ts>>) /\
+      (<<BOUND: forall to fto (MAPPED: f to fto) (TS: Time.lt max to),
+          (Time.lt ts0 fto /\ Time.lt fto ts1)>>) /\
+      (<<MAPLT: mapping_map_lt_loc f>>)
+.
+Proof.
+  hexploit (list_filter_exists (fun ts => Time.lt max ts) T). i. des.
+  hexploit (sorting_sorted l'). i. des.
+  hexploit (@compressing_map_spec ts0 ts1 (sorting l')); eauto. i. des.
+  exists ((fun ts fts => Time.le ts max /\ ts = fts) \2/ (compressing_map ts0 ts1 (sorting l'))).
+  splits.
+
+  - i. destruct (Time.le_lt_dec to max).
+    + esplits; eauto.
+    + hexploit (proj1 (COMPLETE to)).
+      { split; auto. } intros IN'. des.
+      eapply COMPLETE0 in IN'.
+      eapply COMPLETE1 in IN'. des. esplits; eauto.
+  - i. eauto.
+  - i. apply or_strengthen in MAPPED. des; clarify; eauto.
+    + exfalso. eapply Time.lt_strorder. eapply TimeFacts.lt_le_lt; eauto.
+    + eapply BOUND in SAT. des. auto.
+
+  - ii. des; clarify.
+    + apply BOUND in MAP0. des.
+      eapply COMPLETE0 in IN. eapply COMPLETE in IN. des.
+      split; i.
+      * exfalso. eapply Time.lt_strorder. eapply TimeFacts.lt_le_lt.
+        { eapply H. } etrans.
+        { eapply MAP1. }
+        { left. auto. }
+      * exfalso. eapply Time.lt_strorder. eapply TimeFacts.lt_le_lt.
+        { eapply H. } etrans.
+        { eapply MAP1. } etrans.
+        { eapply MAX. }
+        { left. auto. }
+
+    + apply BOUND in MAP1. des.
+      apply COMPLETE0 in IN. eapply COMPLETE in IN. des.
+      split; i.
+      * eapply TimeFacts.le_lt_lt.
+        { eapply MAP0. }
+        eapply TimeFacts.le_lt_lt; eauto.
+      * eapply TimeFacts.le_lt_lt; eauto.
+
+    + eapply MAPLT; eauto.
+Qed.
 
 
-           (space: Loc.t -> Time.t -> Prop)
+Definition pf_consistent_drf_shift lang (e0:Thread.t lang)
+           (spaces: Loc.t -> Time.t -> Prop)
+           (promises: Loc.t -> Time.t -> Prop)
+           (max: TimeMap.t)
+           (U AU: Loc.t -> Prop): Prop :=
+  forall (gap newmax: TimeMap.t)
+         (GAP: forall loc (UPDATES: U loc \/ AU loc),
+             Time.lt (max loc) (gap loc))
+         (NEWMAX: TimeMap.le max newmax),
+  exists e2 tr,
+    (<<STEPS: traced_step tr e0 e2>>) /\
+
+    (<<TRACE: List.Forall (fun em => (no_sc /1\ no_promise /1\ (write_in (spaces \2/ (fun loc to => (__guard__(U loc \/ AU loc) /\ Time.lt (max loc) to /\ Time.lt to (gap loc))) \2/                 (fun loc to => ~ U loc /\ ~ AU loc /\ Time.lt (newmax loc) to)))) (fst em)) tr>>) /\
+
+    (<<COMPLETEU:
+       forall loc (SAT: U loc),
+       exists to from valr valw releasedr releasedw ordr ordw mem,
+         <<IN: List.In (ThreadEvent.update loc from to valr valw releasedr releasedw ordr ordw, mem) tr>> /\ <<ORDR: Ordering.le ordr Ordering.strong_relaxed>> >>) /\
+
+    (<<COMPLETEAU:
+       forall loc (SAT: AU loc),
+       exists to from valr valw releasedr releasedw ordr ordw mem,
+         <<IN: List.In (ThreadEvent.update loc from to valr valw releasedr releasedw ordr ordw, mem) tr>> >>) /\
+
+    (<<COMPLETEW: forall loc to (PROMISED: promises loc to),
+        exists e m,
+          (<<IN: List.In (e, m) tr>>) /\
+          (<<WRITETO: rlx_write_loc loc e>>)>>)
+.
+
+(* TODO: change definition in Pred.v *)
+Definition wf_time_evt (P: Loc.t -> Time.t -> Prop) (e: ThreadEvent.t) : Prop :=
+  match e with
+  | ThreadEvent.promise loc from to msg kind =>
+    (<<FROM: P loc from>>) /\ (<<TO: P loc to>>)
+  | ThreadEvent.write loc from to val released ordw =>
+    (<<FROM: P loc from>>) /\ (<<TO: P loc to>>)
+  | ThreadEvent.update loc from to valr valw releasedr releasedw ordr ordw =>
+    (<<FROM: P loc from>>) /\ (<<TO: P loc to>>)
+  | _ => True
+  end.
+
+Lemma wf_time_evt_mon P0 P1
+      (LE: P0 <2= P1)
+  :
+    wf_time_evt P0 <1= wf_time_evt P1.
+Proof.
+  ii. unfold wf_time_evt in *. des_ifs; des; splits; eauto.
+Qed.
+
+Lemma step_times_list_exists lang (th0 th1: Thread.t lang) e
+      (STEP: AThread.step_allpf e th0 th1)
+  :
+    exists (times: Loc.t -> list Time.t),
+      (<<WFTIME: wf_time_evt (fun loc to => List.In to (times loc)) e>>).
+Proof.
+  destruct e.
+  - exists (fun l => if Loc.eq_dec l loc then
+                       [from; to] else []).
+    econs; eauto.
+    + ss. splits; auto; des_ifs; ss; eauto.
+    + ss. splits; auto; des_ifs; ss; eauto.
+  - exists (fun _ => []). econs; eauto.
+  - exists (fun _ => []). econs; eauto.
+  - exists (fun l => if Loc.eq_dec l loc then
+                       [from; to] else []).
+    econs; eauto.
+    + ss. splits; auto; des_ifs; ss; eauto.
+    + ss. splits; auto; des_ifs; ss; eauto.
+  - exists (fun l => if Loc.eq_dec l loc then
+                       [tsr; tsw] else []).
+    econs; eauto.
+    + ss. splits; auto; des_ifs; ss; eauto.
+    + ss. splits; auto; des_ifs; ss; eauto.
+  - exists (fun _ => []). econs; eauto.
+  - exists (fun _ => []). econs; eauto.
+  - exists (fun _ => []). econs; eauto.
+Qed.
+
+Lemma traced_times_list_exists lang (th0 th1: Thread.t lang) tr
+      (STEPS: traced_step tr th0 th1)
+  :
+    exists (times: Loc.t -> list Time.t),
+      (<<WFTIME: List.Forall (fun em => wf_time_evt (fun loc to => List.In to (times loc)) (fst em)) tr>>).
+Proof.
+  ginduction STEPS.
+  - exists (fun _ => []). econs.
+  - des. eapply step_times_list_exists in HD. des.
+    exists (fun loc => (times0 loc ++ times loc)). econs.
+    + eapply wf_time_evt_mon; eauto.
+      i. ss. eapply List.in_or_app; eauto.
+    + eapply List.Forall_impl; eauto.
+      i. ss. eapply wf_time_evt_mon; eauto.
+      i. ss. eapply List.in_or_app; eauto.
+Qed.
+
+Lemma wf_time_mapped_mappable (tr: list (ThreadEvent.t * Memory.t)) times f
+      (WFTIME: List.Forall (fun em => wf_time_evt (fun loc to => List.In to (times loc)) (fst em)) tr)
+      (COMPLETE: forall loc to (IN: List.In to (times loc)),
+          exists fto, (<<MAPPED: f loc to fto>>))
+  :
+    List.Forall (fun em => mappable_evt f (fst em)) tr.
+Proof.
+  eapply List.Forall_impl; eauto. i. ss. destruct a. destruct t; ss.
+  - des. split.
+    + apply COMPLETE in FROM. des. esplit. eauto.
+    + apply COMPLETE in TO. des. esplit. eauto.
+  - des. split.
+    + apply COMPLETE in FROM. des. esplit. eauto.
+    + apply COMPLETE in TO. des. esplit. eauto.
+  - des. split.
+    + apply COMPLETE in FROM. des. esplit. eauto.
+    + apply COMPLETE in TO. des. esplit. eauto.
+Qed.
+
+(* TODO: unify with ADRF_PF0.v *)
+Lemma step_wf_event lang (th0 th1: Thread.t lang) e
+      (INHABITED: Memory.inhabited th0.(Thread.memory))
+      (STEP: AThread.step_allpf e th0 th1)
+  :
+    wf_event e.
+Proof.
+  inv STEP. inv STEP0.
+  - inv STEP. inv LOCAL. ss.
+    eapply promise_wf_event; eauto.
+  - inv STEP. inv LOCAL; ss.
+    + inv LOCAL0. eapply write_wf_event; eauto.
+    + inv LOCAL1. inv LOCAL2. eapply write_wf_event; eauto.
+Qed.
+
+(* TODO: unify with ADRF_PF0.v *)
+Lemma traced_step_wf_event lang (th0 th1: Thread.t lang) tr
+      (INHABITED: Memory.inhabited th0.(Thread.memory))
+      (STEPS: traced_step tr th0 th1)
+  :
+    List.Forall (fun em => wf_event (fst em)) tr.
+Proof.
+  ginduction STEPS; i.
+  - econs.
+  - econs.
+    + eapply step_wf_event; eauto.
+    + eapply IHSTEPS. inv HD. eapply AThread.step_inhabited; eauto.
+Qed.
+
+
+Lemma pf_consistent_drf_src_shift lang (e0: Thread.t lang) spaces promises max U AU
+      (LOCAL: Local.wf (Thread.local e0) (Thread.memory e0))
+      (SC: Memory.closed_timemap (Thread.sc e0) (Thread.memory e0))
+      (CLOSED: Memory.closed (Thread.memory e0))
+      (CONSISTENT: pf_consistent_drf_src e0 spaces promises max U AU)
+  :
+    pf_consistent_drf_shift e0 spaces promises max U AU.
+Proof.
+  ii. unfold pf_consistent_drf_src in CONSISTENT. des.
+  exploit (choice
+             (fun loc to =>
+                forall (SAT: MU loc),
+                  (<<NOTUPDATES: ~ U loc /\ ~ AU loc>>) /\
+                  (<<TS0: Time.le (Memory.max_ts loc e0.(Thread.memory)) to>>) /\
+                  (<<TS1: Time.lt to (max loc)>>) /\
+                  (<<BLANK: Interval.mem (to, (max loc)) <1= spaces loc>>))).
+  { intros loc. destruct (classic (MU loc)).
+    - eapply MYUPDATES in H. des. exists to. esplits; eauto.
+    - exists Time.bot. i. clarify. }
+  i. clear MYUPDATES. destruct x0 as [mu MYUPDATES].
+
+  exploit traced_times_list_exists; eauto. i. des.
+  exploit (choice
+             (fun loc (floc: Time.t -> Time.t -> Prop) =>
+                (<<COMPLETE: forall to (IN: List.In to (times loc)),
+                    exists fto, (<<MAPPED: floc to fto>>)>>) /\
+                (<<NUS: forall (SAT: ~ U loc /\ ~ AU loc /\ ~ MU loc),
+                    (<<SAME: forall ts (TS: Time.le ts (max loc)), floc ts ts>>) /\
+                    (<<MAPGAP: exists fts, <<MAPPED: floc (max' loc) fts>> /\ Time.lt (newmax loc) fts>>) /\
+                    (<<RANGE: forall ts fts (MAPPED: floc ts fts) (TS: Time.lt (max loc) ts),
+                        Time.lt (newmax loc) fts>>)>>) /\
+                (<<UAUS: forall (SAT: __guard__(U loc \/ AU loc)),
+                    (<<SAME: forall ts (TS: Time.le ts (max loc)), floc ts ts>>) /\
+                    (<<RANGE: forall ts fts (MAPPED: floc ts fts) (TS: Time.lt (max loc) ts),
+                        Time.lt (max loc) fts /\ Time.lt fts (gap loc)>>)>>) /\
+                (<<MUS: forall (SAT: MU loc),
+                    (<<SAME: forall ts (TS: Time.le ts (mu loc)), floc ts ts>>) /\
+                    (<<RANGE: forall ts fts (MAPPED: floc ts fts) (TS: Time.lt (mu loc) ts),
+                        Time.lt (mu loc) fts /\ Time.lt fts (max loc)>>)>>) /\
+                (<<MAPLT: mapping_map_lt_loc floc>>)
+          )).
+  { intros loc. destruct (classic (MU loc)).
+    { exploit MYUPDATES; eauto. i. des.
+      exploit (@shift_map_exists (mu loc) (mu loc) (max loc)); auto.
+      { refl. }
+      i. des. esplits; eauto; i; des; clarify.
+      exfalso. unguard. des; clarify.
+    }
+    destruct (classic (__guard__(U loc \/ AU loc))).
+    { exploit (@shift_map_exists (max loc) (max loc) (gap loc)); auto.
+      { refl. }
+      i. des. esplits; eauto; i.
+      - clarify. unguard. exfalso. des; eauto.
+      - exploit MYUPDATES; eauto. i. des. unguard. des; clarify. }
+    { exploit (@shift_map_exists (max loc) (newmax loc) (Time.incr (newmax loc)) ((max' loc)::(times loc))); auto.
+      { apply Time.incr_spec. }
+      i. des. esplits; eauto; i; clarify.
+      { eapply COMPLETE; eauto. ss. auto. } splits; auto.
+      { ss. exploit COMPLETE; eauto. i. des. esplits; eauto.
+        exploit BOUND; eauto. i. des. auto. }
+      i. exploit BOUND; eauto. i. des; auto.
+    }
+  }
+  intros [f FSPEC].
+
+  assert (MAPLT: mapping_map_lt f).
+  { eapply mapping_map_lt_locwise. i. specialize (FSPEC loc). des. auto. }
+  assert (IDENTINMAP: map_ident_in_memory f (Thread.memory e0)).
+  { ii. specialize (FSPEC loc). des.
+    destruct (classic (MU loc)).
+    { exploit MUS; eauto. i. des.
+      exploit MYUPDATES; eauto. i. des.
+      eapply SAME. etrans; eauto. }
+    destruct (classic (__guard__(U loc \/ AU loc))).
+    { exploit UAUS; eauto. i. des.
+      eapply SAME. etrans; eauto. }
+    { exploit NUS; eauto.
+      { unguard. apply not_or_and in H0. des. split; auto. }
+      i. des.
+      eapply SAME. etrans; eauto. }
+  }
+  assert (MAPEQ: mapping_map_eq f).
+  { eapply mapping_map_lt_map_eq; eauto. }
+
+  assert (MAPPABLE: List.Forall (fun em => mappable_evt f (fst em)) tr).
+  { eapply wf_time_mapped_mappable; eauto. i.
+    specialize (FSPEC loc). des.
+    destruct (classic (MU loc)).
+    { exploit MUS; eauto. }
+    destruct (classic (__guard__(U loc \/ AU loc))).
+    { exploit UAUS; eauto. }
+    { exploit NUS; eauto.
+      unguard. apply not_or_and in H0. des. split; auto. }
+  }
+
+  exploit traced_step_wf_event; eauto.
+  { inv CLOSED. auto. } intros WFEVT.
+
+  destruct e0 as [st0 lc0 sc0 mem0].
+  destruct e2 as [st1 lc1 sc1 mem1]. ss.
+  hexploit traced_steps_map; try apply STEPS; eauto.
+  { eapply mapping_map_lt_map_le; eauto. }
+  { eapply map_ident_in_memory_bot; eauto. }
+  { eapply map_ident_in_memory_local; eauto. }
+  { eapply map_ident_in_memory_memory; eauto. }
+  { eapply mapping_map_lt_collapsable_unwritable; eauto. }
+  { eapply map_ident_in_memory_closed_timemap; eauto. }
+  { refl. }
+  i. des. esplits; eauto.
+
+  - eapply List.Forall_forall. i.
+    eapply list_Forall2_in in H; eauto. des. destruct a, x. ss.
+    eapply List.Forall_forall in TRACE; eauto. ss. des.
+    eapply List.Forall_forall in WFEVT; eauto. ss.
+    inv EVENT; ss.
+
+    + splits; auto.
+      specialize (FSPEC loc). des.
+      destruct (classic (MU loc)).
+      { exploit MUS; eauto. i. des.
+        exploit MYUPDATES; eauto. i. des.
+        destruct (Time.le_lt_dec to (mu loc)).
+        - left. left. exploit SAME.
+          { instantiate (1:=from). etrans.
+            { left. eauto. }
+            { eauto. } } intros MAPFROM.
+          exploit SAME.
+          { eapply l. } intros MAPTO.
+          hexploit (MAPEQ _ _ _ _ MAPTO TO). i. subst.
+          hexploit (MAPEQ _ _ _ _ MAPFROM FROM). i. subst.
+          hexploit (TRACE1 t); eauto. i. des; auto.
+          { unfold later_times in H0.
+            exfalso. eapply Time.lt_strorder. eapply TimeFacts.lt_le_lt.
+            { eapply H0. }
+            etrans; eauto. etrans.
+            { inv IN0. eauto. } etrans; eauto.
+            left. auto. }
+        - left.
+          admit.
+      }
+
+      destruct (classic (__guard__(U loc \/ AU loc))).
+      { exploit UAUS; eauto. i. des.
+
+
+      }
+      { exploit NUS; eauto.
+        unguard. apply not_or_and in H0. des. split; auto. }
+  }
+
+
+
+              left. eauto. }
+            eauto. }
+          left. left.
+
+
+          { econs; ss. refl. } i. des.
+          { unfold later_times in H0.
+            exfalso. eapply Time.lt_strorder. eapply TimeFacts.lt_le_lt.
+            { eapply H0. }
+            etrans; eauto. etrans.
+            { left. eauto. }
+            eauto. }
+          left. left.
+
+          exploit SAME.
+          { instantiate (1:=from). etrans.
+            { left. eauto. }
+            { eauto. } } intros MAPFROM.
+          exploit SAME.
+          { eapply l. } intros MAPTO.
+          hexploit (MAPEQ _ _ _ _ MAPTO TO). i. subst.
+          left.
+
+            instantiate (1:=from). etrans.
+            { left. eauto. }
+            { eauto. } } intros MAPFROM.
+
+
+            from
+
+
+        - admit.
+
+        -
+
+        - left. left.
+
+        Lemma s: True.
+
+
+      }
+      destruct (classic (__guard__(U loc \/ AU loc))).
+      { exploit UAUS; eauto. }
+      { exploit NUS; eauto.
+        unguard. apply not_or_and in H0. des. split; auto. }
+
+
+      intros ts. dest
+
+    destruct b. ss.
+
+    admit.
+
+  - i. eapply COMPLETEU in SAT. des.
+    eapply list_Forall2_in2 in IN; eauto. des. ss. destruct b. ss.
+    inv EVENT. esplits; eauto.
+
+  - i. eapply COMPLETEAU in SAT. des.
+    eapply list_Forall2_in2 in IN; eauto. des. ss. destruct b. ss.
+    inv EVENT. esplits; eauto.
+
+  - i. eapply COMPLETEW in PROMISED. des.
+    eapply list_Forall2_in2 in IN; eauto. des. ss. destruct b. ss.
+    inv EVENT; ss.
+    + esplits; eauto.
+    + esplits; eauto.
+
+Qed.
+
+  Lemma sorting_sorted l
+    :
+      (<<COMPLETE: forall a, List.In a l <-> List.In a (sorting l)>>) /\
+      (<<SORTED: times_sorted (sorting l)>>).
+  Proof.
+    induction l; ss.
+    - split; i; ss.
+    - i. des. splits.
+      + i. erewrite insert_complete.
+        split; i; des; eauto.
+        * right. eapply COMPLETE; eauto.
+        * right. eapply COMPLETE; eauto.
+      + eapply insert_sorted; eauto.
+  Qed.
+
+
+
+  Lemma sorting_sorted l
+    :
+      (<<COMPLETE: forall a, List.In a l <-> List.In a (sorting l)>>) /\
+      (<<SORTED: times_sorted (sorting l)>>).
+  Proof.
+    induction l; ss.
+    - split; i; ss.
+    - i. des. splits.
+      + i. erewrite insert_complete.
+        split; i; des; eauto.
+        * right. eapply COMPLETE; eauto.
+        * right. eapply COMPLETE; eauto.
+      + eapply insert_sorted; eauto.
+  Qed.
+
+
+Lemma shift_map_exists f0 t0 t1
+      (TS: Time.lt t0 t1)
+      (MAPLT0: mapping_map_lt_loc f)
+  :
+    forall (T: list Time.t),
+    exists (f: Time.t -> Time.t -> Prop),
+      (<<COMPLETE: forall to (IN: List.In to T), exists fto, (<<MAPPED: f to fto>>)>>) /\
+      (<<ONLY: forall to fto (MAPPED: f to fto),
+          (<<TS: Time.le to t0>>) \/ (<<IN: List.In to T>>)>>) /\
+      (<<SAME: forall ts (TS: Time.le ts t0), f ts ts>>) /\
+      (<<BOUND: forall to fto (MAPPED: f to fto), Time.lt fto t1>>) /\
+      (<<MAPLT: mapping_map_lt_loc f>>)
+
+
+Lemma shift_map_exists f0 t0 t1
+      (TS: Time.lt t0 t1)
+      (MAPLT0: mapping_map_lt_loc f)
+  :
+    forall (T: list Time.t),
+    exists (f: Time.t -> Time.t -> Prop),
+      (<<COMPLETE: forall to (IN: List.In to T), exists fto, (<<MAPPED: f to fto>>)>>) /\
+      (<<ONLY: forall to fto (MAPPED: f to fto),
+          (<<TS: Time.le to t0>>) \/ (<<IN: List.In to T>>)>>) /\
+      (<<SAME: forall ts (TS: Time.le ts t0), f ts ts>>) /\
+      (<<BOUND: forall to fto (MAPPED: f to fto), Time.lt fto t1>>) /\
+      (<<MAPLT: mapping_map_lt_loc f>>)
+
+
+  :
+    exists (f: Time.t -> Time.t -> Prop),
+      (<<COMPLETE: forall to (IN: List.In to T), exists fto, (<<MAPPED: f to fto>>)>>) /\
+      (<<ONLY: forall to fto (MAPPED: f to fto),
+          (<<TS: Time.le to t0>>) \/ (<<IN: List.In to T>>)>>) /\
+      (<<SAME: forall ts (TS: Time.le ts t0), f ts ts>>) /\
+      (<<BOUND: forall to fto (MAPPED: f to fto), Time.lt fto t1>>) /\
+      (<<MAPLT: mapping_map_lt_loc f>>)
+.
+Proof.
+  ginduction T.
+  - i. exists (fun to fto => to = fto /\ Time.le to t0). splits.
+    + i. inv IN.
+    + i. des; auto.
+    + i. split; auto.
+    + i. des. subst. eapply TimeFacts.le_lt_lt; eauto.
+    + ii. des. subst. auto.
+
+  - i. exploit IHT; eauto. i. des. clear IHT.
+
+    destruct (Time.le_lt_dec a t0).
+    { exists f. splits; auto.
+      - i. ss. des; eauto. subst. esplits. eapply SAME. auto.
+      - i. eapply ONLY in MAPPED. ss. des; auto. }
+
+    destruct (classic (List.In a T)).
+    { exists f. splits; auto.
+      - i. ss. des; subst; eauto.
+      - i. ss. eapply ONLY in MAPPED. des; auto. }
+
+
+
+Lemma compress_map_exists t0 t1 (T: list Time.t)
+      (TS: Time.lt t0 t1)
+  :
+    exists (f: Time.t -> Time.t -> Prop),
+      (<<COMPLETE: forall to (IN: List.In to T), exists fto, (<<MAPPED: f to fto>>)>>) /\
+      (<<ONLY: forall to fto (MAPPED: f to fto),
+          (<<TS: Time.le to t0>>) \/ (<<IN: List.In to T>>)>>) /\
+      (<<SAME: forall ts (TS: Time.le ts t0), f ts ts>>) /\
+      (<<BOUND: forall to fto (MAPPED: f to fto), Time.lt fto t1>>) /\
+      (<<MAPLT: mapping_map_lt_loc f>>)
+.
+Proof.
+  ginduction T.
+  - i. exists (fun to fto => to = fto /\ Time.le to t0). splits.
+    + i. inv IN.
+    + i. des; auto.
+    + i. split; auto.
+    + i. des. subst. eapply TimeFacts.le_lt_lt; eauto.
+    + ii. des. subst. auto.
+
+  - i. exploit IHT; eauto. i. des. clear IHT.
+
+    destruct (Time.le_lt_dec a t0).
+    { exists f. splits; auto.
+      - i. ss. des; eauto. subst. esplits. eapply SAME. auto.
+      - i. eapply ONLY in MAPPED. ss. des; auto. }
+
+    destruct (classic (List.In a T)).
+    { exists f. splits; auto.
+      - i. ss. des; subst; eauto.
+      - i. ss. eapply ONLY in MAPPED. des; auto. }
+
+
+    exploit (fun ts => Time.l
+
+
+      Lemma finite_greatest P (l: list Time.t)
+    :
+      (exists to,
+          (<<SAT: P to>>) /\
+          (<<IN: List.In to l>>) /\
+          (<<GREATEST: forall to'
+                              (IN: List.In to' l)
+                              (SAT: P to'),
+              Time.le to' to>>)) \/
+      (<<EMPTY: forall to (IN: List.In to l), ~ P to>>).
+
+
+
+      etrans; eauto.
+
+
+
+      (<<BOUND: forall ts
+
+
+
+                          exists fto, (<<MAPPED: f loc to fto>>)
 
 
 
 
 
-                                                         Prop :=
 
 
-  let L := (fun loc => Memory.latest_reserve loc e0.(Thread.local).(Local.promises) e0.(Thread.memory)) in
-  forall mem1 max sc
-         (FORGET: forget_memory (latest_other_reserves e0.(Thread.local).(Local.promises) e0.(Thread.memory)) mem1 e0.(Thread.memory))
-         (MAX: my_max_timemap e0.(Thread.local).(Local.promises) e0.(Thread.memory) max),
-  exists e1,
-    (<<STEPS0: rtc (tau (@pred_step ((promise_free /1\ no_acq_update_on ((fun loc to => L loc) /2\ Memory.max_full_ts e0.(Thread.memory))) /1\ no_sc /1\ write_in (later_times max \2/ fun loc to => covered loc to e0.(Thread.local).(Local.promises))) lang)) (Thread.mk _ e0.(Thread.state) e0.(Thread.local) sc mem1) e1>>) /\
-    (__guard__((<<FAILURE: Local.failure_step e1.(Thread.local)>>) \/
-               (<<PROMISES: e1.(Thread.local).(Local.promises) = Memory.bot>>))).
+Lemma ident_map_local
+      lc
+  :
+    local_map ident_map lc lc.
+Proof.
+  econs; i.
+  - refl.
+  - econs; i; eapply ident_map_view.
+  - eapply ident_map_promises.
+Qed.
+
+
+Definition mapping_map_lt_loc (f: Time.t -> Time.t -> Prop):=
+  forall t0 t1 ft0 ft1
+         (MAP0: f t0 ft0)
+         (MAP1: f t1 ft1),
+    Time.lt t0 t1 <-> Time.lt ft0 ft1.
+
+Lemma mapping_map_lt_locwise f
+      (MAPLT: forall loc, mapping_map_lt_loc (f loc))
+  :
+    mapping_map_lt f.
+Proof.
+  ii. eapply MAPLT; eauto.
+
+
+
+
+Lemma ident_map_bot
+  :
+    mapping_map_bot ident_map.
+Proof.
+  unfold ident_map in *. ii. clarify.
+Qed.
+
+Lemma ident_map_eq
+  :
+    mapping_map_eq ident_map.
+Proof.
+  unfold ident_map in *. ii. clarify.
+Qed.
+
+Lemma ident_map_total
+      loc to
+  :
+    exists fto,
+      <<MAP: ident_map loc to fto >>.
+Proof.
+  esplits; eauto. refl.
+Qed.
+
+Lemma mapping_map_lt_non_collapsable f
+      (MAPLT: mapping_map_lt f)
+      loc to
+  :
+    non_collapsable f loc to.
+Proof.
+  ii. unfold collapsed in *. des.
+  eapply MAPLT in TLE; eauto. eapply Time.lt_strorder; eauto.
+Qed.
+
+Lemma ident_map_timemap
+      tm
+  :
+    timemap_map ident_map tm tm.
+Proof.
+  ii. refl.
+Qed.
+
+Lemma ident_map_view
+      vw
+  :
+    view_map ident_map vw vw.
+Proof.
+  econs; eapply ident_map_timemap.
+Qed.
+
+Lemma ident_map_message
+      msg
+  :
+    msg_map ident_map msg msg.
+Proof.
+  destruct msg; econs. destruct released; econs.
+  apply ident_map_view.
+Qed.
+
+Lemma ident_map_promises
+      prom
+  :
+    promises_map ident_map prom prom.
+Proof.
+  econs; i.
+  - esplits; eauto.
+    + eapply mapping_map_lt_non_collapsable.
+      eapply ident_map_lt.
+    + refl.
+    + eapply ident_map_message.
+  - esplits; eauto; refl.
+Qed.
+
+Lemma ident_map_local
+      lc
+  :
+    local_map ident_map lc lc.
+Proof.
+  econs; i.
+  - refl.
+  - econs; i; eapply ident_map_view.
+  - eapply ident_map_promises.
+Qed.
+
+Lemma mapping_map_lt_collapsable_unwritable f prom mem
+      (MAPLT: mapping_map_lt f)
+  :
+    collapsable_unwritable f prom mem.
+Proof.
+  ii. exfalso. des.
+  eapply mapping_map_lt_non_collapsable; try eassumption.
+  inv ITV. eapply TimeFacts.lt_le_lt; eauto.
+Qed.
+
+
+Lemma mapping_map_lt_map_le f
+      (MAPLT: forall loc, mapping_map_lt_loc (f loc))
+      (MAPLE: forall loc, mapping_map_lt_loc (f loc))
+  :
+    mapping_map_le f.
+Proof.
+  ii.
+
+
+Definition mapping_map_lt_loc (f: Time.t -> Time.t -> Prop):=
+  forall t0 t1 ft0 ft1
+         (MAP0: f t0 ft0)
+         (MAP1: f t1 ft1),
+    Time.lt t0 t1 -> Time.lt ft0 ft1.
+
+Lemma mapping_map_lt_map_le f
+      (MAPLT: forall loc, mapping_map_lt_loc (f loc))
+      (MAPLE: forall loc, mapping_map_lt_loc (f loc))
+  :
+    mapping_map_le f.
+Proof.
+  ii.
+
+Definition pf_consistent_drf_src_future lang (e0:Thread.t lang)
+           (spaces: Loc.t -> Time.t -> Prop)
+           (promises: Loc.t -> Time.t -> Prop)
+           (max: TimeMap.t)
+           (U AU: Loc.t -> Prop): Prop :=
+  forall
+
+  exists e2 tr max',
+
+
+
+    (<<STEPS: traced_step tr e0 e2>>) /\
+    (<<MAX: TimeMap.le e0.(Thread.memory).(Memory.max_timemap) max>>) /\
+    (<<SPACES: spaces <2= earlier_times max>>) /\
+
+    (<<TIMEMAP: TimeMap.le max max'>>) /\
+    (<<GAP: forall loc (NUPDATES: ~ U loc /\ ~ AU loc /\ ~ MU loc),
+        Time.lt (max loc) (max' loc)>>) /\
+
+    (<<TRACE: List.Forall (fun em => (no_sc /1\ no_promise /1\ (write_in (later_times max' \2/ (spaces /2\ earlier_times max)))) (fst em)) tr>>) /\
+
+    (<<COMPLETEU:
+       forall loc (SAT: U loc),
+       exists to from valr valw releasedr releasedw ordr ordw mem,
+         <<IN: List.In (ThreadEvent.update loc from to valr valw releasedr releasedw ordr ordw, mem) tr>> /\ <<ORDR: Ordering.le ordr Ordering.strong_relaxed>> >>) /\
+
+    (<<COMPLETEAU:
+       forall loc (SAT: AU loc),
+       exists to from valr valw releasedr releasedw ordr ordw mem,
+         <<IN: List.In (ThreadEvent.update loc from to valr valw releasedr releasedw ordr ordw, mem) tr>> >>) /\
+
+    (<<MYUPDATES: forall loc (SAT: MU loc),
+        exists to,
+          (<<TS0: Time.le (Memory.max_ts loc e0.(Thread.memory)) to>>) /\
+          (<<TS1: Time.lt to (max loc)>>) /\
+          (<<BLANK: Interval.mem (to, (max loc)) <1= spaces loc>>)>>) /\
+
+    (<<COMPLETEW: forall loc to (PROMISED: promises loc to),
+        exists e m,
+          (<<IN: List.In (e, m) tr>>) /\
+          (<<WRITETO: rlx_write_loc loc e>>)>>)
+.
+
+
+
+
+(* Inductive shifted_map mlast mcert *)
+(*           (updates: Loc.t -> Prop) *)
+(*           (sky gap: TimeMap.t) *)
+(*           (f: Loc.t -> Time.t -> Time.t): Prop := *)
+(* | shifted_map_intro *)
+(*     (PRSV: map_preserving (times_in_memory mcert) f) *)
+(*     (SAME: forall l t (TLE: Time.le t (Memory.max_ts l mlast)), *)
+(*         f l t = t) *)
+(*     (INGAP: forall l t (TLT: Time.lt (Memory.max_ts l mcert) t), *)
+(*         Time.lt (f l t) (gap l)) *)
+(*     (AFTERSKY: forall l t (TLT: Time.lt (Memory.max_ts l mcert) t), *)
+(*         Time.lt (sky l) (f l t)) *)
+(* . *)
+
+(* Lemma shifted_map_exists mlast mcert updates *)
+(*       (MLE: Memory.le mlast mcert) *)
+(*       (sky gap: TimeMap.t) *)
+(*       (SKY: forall l, Time.lt (Memory.max_ts l mlast) (sky l)) *)
+(*       (GAP: forall l, Time.lt (Memory.max_ts l mlast) (gap l)) *)
+(*   : *)
+(*     exists f, (<<SHIFTED: shifted_map mlast mcert updates sky gap f>>). *)
+(* Proof. *)
+(*   (* may be very hard... *) *)
+(* Admitted. *)
+
+(* Lemma shifted_map_preserving_last_mem  mlast mcert updates sky gap f *)
+(*       (CLOSED: Memory.closed mlast) *)
+(*       (SHIFTED: shifted_map mlast mcert updates sky gap f) *)
+(*   : *)
+(*     memory_map f mlast mlast. *)
+(* Proof. *)
+(*   inv SHIFTED. inv PRSV. econs; i. *)
+(*   - exploit Memory.max_ts_spec; eauto. i. des. *)
+(*     repeat erewrite SAME; eauto. *)
+(*     + rewrite GET. unfold msg_map. des_ifs. repeat f_equal. *)
+(*       inv CLOSED. exploit CLOSED0; try apply GET; eauto. i. des. *)
+(*       inv MSG_CLOSED. inv CLOSED; ss. f_equal. *)
+(*       destruct view. inv CLOSED1. unfold view_map, timemap_map. ss. f_equal. *)
+(*       * extensionality l. erewrite SAME; auto. *)
+(*         specialize (PLN l). des. *)
+(*         exploit Memory.max_ts_spec; eauto. i. des. auto. *)
+(*       * extensionality l. erewrite SAME; auto. *)
+(*         specialize (RLX l). des. *)
+(*         exploit Memory.max_ts_spec; eauto. i. des. auto. *)
+(*     + exploit Memory.get_ts; try apply GET; eauto. i. des. *)
+(*       * clarify. *)
+(*       * left. eapply TimeFacts.lt_le_lt; eauto. *)
+(*   - destruct msg_src as [from msg]. exploit Memory.max_ts_spec; eauto. i. des. *)
+(*     esplits. *)
+(*     + erewrite SAME; eauto. *)
+(*     + eauto. *)
+(* Qed. *)
